Aesop/Search/Expansion/Simp.lean
@@ -29,81 +29,69 @@ end SimpResult
 
 variable [Monad m] [MonadQuotation m] [MonadError m]
 
--- TODO copy-pasta from Lean.Elab.Tactic.traceSimpCall
--- NOTE: Must be executed in the context of the goal on which `simp` was run.
+-- Copy-pasta from Lean.Elab.Tactic.traceSimpCall.
 -- `stx` is the syntax of the original `simp`/`simp_all`/`simp?`/`simp_all?`
 -- call.
-def mkSimpOnly (stx : Syntax) (usedSimps : UsedSimps) (includeFVars : Bool) :
-    MetaM Syntax := do
-  let mut stx := stx
-  if stx[3].isNone then
-    stx := stx.setArg 3 (mkNullNode #[mkAtom "only"])
-  let mut args : Array Syntax := #[]
-  let mut localsOrStar := some #[]
-  let lctx ← getLCtx
-  let env ← getEnv
-  for (thm, _) in usedSimps.toArray.qsort (·.2 < ·.2) do
-    match thm with
-    | .decl declName inv => -- global definitions in the environment
-      if env.contains declName && !Lean.Elab.Tactic.simpOnlyBuiltins.contains declName then
-        args := args.push (← if inv then
-          `(Parser.Tactic.simpLemma| ← $(mkIdent (← unresolveNameGlobal declName)):ident)
-        else
-          `(Parser.Tactic.simpLemma| $(mkIdent (← unresolveNameGlobal declName)):ident))
-    | .fvar fvarId => -- local hypotheses in the context
-      if ! includeFVars then
-        continue
-      if let some ldecl := lctx.find? fvarId then
-        localsOrStar := localsOrStar.bind fun locals =>
-          if !ldecl.userName.isInaccessibleUserName &&
-              (lctx.findFromUserName? ldecl.userName).get!.fvarId == ldecl.fvarId then
-            some (locals.push ldecl.userName)
+def mkSimpOnly (inGoal : MVarId) (stx : Syntax) (usedSimps : UsedSimps)
+    (includeFVars : Bool) : MetaM Syntax :=
+  inGoal.withContext do
+    let mut stx := stx
+    if stx[3].isNone then
+      stx := stx.setArg 3 (mkNullNode #[mkAtom "only"])
+    let mut args : Array Syntax := #[]
+    let mut localsOrStar := some #[]
+    let lctx ← getLCtx
+    let env ← getEnv
+    for (thm, _) in usedSimps.toArray.qsort (·.2 < ·.2) do
+      match thm with
+      | .decl declName inv => -- global definitions in the environment
+        if env.contains declName && !Lean.Elab.Tactic.simpOnlyBuiltins.contains declName then
+          args := args.push (← if inv then
+            `(Parser.Tactic.simpLemma| ← $(mkIdent (← unresolveNameGlobal declName)):ident)
           else
-            none
-      -- Note: the `if let` can fail for `simp (config := {contextual := true})` when
-      -- rewriting with a variable that was introduced in a scope. In that case we just ignore.
-    | .stx _ thmStx => -- simp theorems provided in the local invocation
-      args := args.push thmStx
-    | .other _ => -- Ignore "special" simp lemmas such as constructed by `simp_all`.
-      pure ()     -- We can't display them anyway.
-  if let some locals := localsOrStar then
-    args := args ++ (← locals.mapM fun id => `(Parser.Tactic.simpLemma| $(mkIdent id):ident))
-  else
-    args := args.push (← `(Parser.Tactic.simpStar| *))
-  let argsStx := if args.isEmpty then #[] else #[mkAtom "[", (mkAtom ",").mkSep args, mkAtom "]"]
-  stx := stx.setArg 4 (mkNullNode argsStx)
-  return stx
+            `(Parser.Tactic.simpLemma| $(mkIdent (← unresolveNameGlobal declName)):ident))
+      | .fvar fvarId => -- local hypotheses in the context
+        if ! includeFVars then
+          continue
+        if let some ldecl := lctx.find? fvarId then
+          localsOrStar := localsOrStar.bind fun locals =>
+            if !ldecl.userName.isInaccessibleUserName &&
+                (lctx.findFromUserName? ldecl.userName).get!.fvarId == ldecl.fvarId then
+              some (locals.push ldecl.userName)
+            else
+              none
+        -- Note: the `if let` can fail for `simp (config := {contextual := true})` when
+        -- rewriting with a variable that was introduced in a scope. In that case we just ignore.
+      | .stx _ thmStx => -- simp theorems provided in the local invocation
+        args := args.push thmStx
+      | .other _ => -- Ignore "special" simp lemmas such as constructed by `simp_all`.
+        pure ()     -- We can't display them anyway.
+    if let some locals := localsOrStar then
+      args := args ++ (← locals.mapM fun id => `(Parser.Tactic.simpLemma| $(mkIdent id):ident))
+    else
+      args := args.push (← `(Parser.Tactic.simpStar| *))
+    let argsStx := if args.isEmpty then #[] else #[mkAtom "[", (mkAtom ",").mkSep args, mkAtom "]"]
+    stx := stx.setArg 4 (mkNullNode argsStx)
+    return stx
 
--- TODO this way to handle (config := ...) is ugly.
-def mkNormSimpSyntax (normSimpUseHyps : Bool)
-    (configStx? : Option Term) : MetaM Syntax.Tactic := do
-  if normSimpUseHyps then
+def mkNormSimpSyntax (useHyps : Bool) (configStx? : Option Term) :
+    MetaM Syntax.Tactic := do
+  if useHyps then
     match configStx? with
     | none => `(tactic| simp_all)
-    | some cfg =>
-      `(tactic| simp_all (config := ($cfg : Aesop.SimpConfig).toConfigCtx))
+    | some cfg => `(tactic| simp_all (config := $cfg))
   else
     match configStx? with
     | none => `(tactic| simp at *)
-    | some cfg =>
-      `(tactic| simp (config := ($cfg : Aesop.SimpConfig).toConfig) at *)
+    | some cfg => `(tactic| simp (config := $cfg) at *)
 
-def mkNormSimpOnlySyntax (inGoal : MVarId) (normSimpUseHyps : Bool)
+def mkNormSimpOnlySyntax (inGoal : MVarId) (useHyps : Bool)
     (configStx? : Option Term) (usedTheorems : Simp.UsedSimps) :
     MetaM Syntax.Tactic := do
-  let originalStx ← mkNormSimpSyntax normSimpUseHyps configStx?
-  let includeFVars := ! normSimpUseHyps
-  let stx ← inGoal.withContext do
-    mkSimpOnly originalStx usedTheorems (includeFVars := includeFVars)
+  let originalStx ← mkNormSimpSyntax useHyps configStx?
+  let stx ←
+    mkSimpOnly inGoal originalStx usedTheorems (includeFVars := ! useHyps)
   return ⟨stx⟩
-
-def mkNormSimpContext (rs : RuleSet) (simpConfig : Aesop.SimpConfig) :
-    MetaM Simp.Context :=
-  return {
-    ← Simp.Context.mkDefault with
-    simpTheorems := #[rs.normSimpLemmas]
-    config := simpConfig.toConfig
-  }
 
 def simpGoal (mvarId : MVarId) (ctx : Simp.Context)
     (discharge? : Option Simp.Discharge := none)
@@ -121,18 +109,12 @@ def simpGoal (mvarId : MVarId) (ctx : Simp.Context)
   else
     return .solved usedSimps
 
-def simpGoalWithAllHypotheses (mvarId : MVarId) (ctx : Simp.Context)
+def simpAtStar (mvarId : MVarId) (ctx : Simp.Context)
     (discharge? : Option Simp.Discharge := none)
     (simplifyTarget : Bool := true) (usedSimps : UsedSimps := {}) :
-    MetaM SimpResult :=
-  mvarId.withContext do
-    let lctx ← getLCtx
-    let mut fvarIdsToSimp := Array.mkEmpty lctx.decls.size
-    for ldecl in lctx do
-      if ldecl.isImplementationDetail then
-        continue
-      fvarIdsToSimp := fvarIdsToSimp.push ldecl.fvarId
-    Aesop.simpGoal mvarId ctx discharge? simplifyTarget fvarIdsToSimp usedSimps
+    MetaM SimpResult := do
+  let fvarIdsToSimp ← mvarId.getNondepPropHyps
+  Aesop.simpGoal mvarId ctx discharge? simplifyTarget fvarIdsToSimp usedSimps
 
 def simpAll (mvarId : MVarId) (ctx : Simp.Context)
     (usedSimps : UsedSimps := {}) : MetaM SimpResult := do
