tests/ElabConfig.lean
@@ -12,4 +12,4 @@ example : True := by
   aesop (options := { noSuchOption := true })
 
 example : True := by
-  aesop (simp_options := { noSuchOption := true })
+  aesop (simp_config := { noSuchOption := true })
